commit before merge

examples/refinement/layering/LowStar.Lens.DependentMap.fst
@@ -4,8 +4,11 @@ open LowStar.Lens
 open FStar.HyperStack.ST
 open FStar.Tactics
 open FStar.BigOps
-  
-module DM = FStar.DependentGMap
+open FStar.Classical 
+
+module DGM = FStar.DependentGMap
+module DM = FStar.DependentMap
+
 module B = LowStar.Buffer
 module HS = FStar.HyperStack
 module HST = FStar.HyperStack.ST
@@ -27,8 +30,9 @@ module List = FStar.List.Tot.Base
 //   List.map (fun k -> (| k,  DM.sel m k |)) dom 
 
 // all pointers in a heap are live in a given mem 
+unfold
 let map_inv (#t:eqtype) (f: t -> Type) (m:DM.t t (fun (x:t) -> B.pointer (f x))) (dom:list t) (h : HS.mem) : Type0 =
-  big_and #t (fun x -> B.live h (DM.sel m x)) dom
+  big_and' #t (fun x -> B.live h (DM.sel m x)) dom
 
 // locations of a dependent map
 let rec map_loc (#t:eqtype) (f: t -> Type) (m:DM.t t (fun (x:t) -> B.pointer (f x))) (dom:list t) : GTot B.loc =
@@ -38,6 +42,11 @@ match dom with
 
 // Union of locations in a pointer list
 let map_eloc #t f m dom : eloc = Ghost.hide (map_loc #t f m dom)
+
+// Lemmas about map_inv
+let map_inv_mem (#t:eqtype) (f: t -> Type) (m:DM.t t (fun (x:t) -> B.pointer (f x)))
+   (dom:list t) (h : imem (map_inv f m dom)) (x:t{List.memP x dom}) : Lemma (B.live h (DM.sel m x)) =
+   let p = big_and'_forall #t (fun x -> B.live h (DM.sel m x)) dom in ()
 
 (* Preservation of liveness after memory updates *)
 
@@ -76,6 +85,40 @@ let dom (#a:eqtype) (lst:list a) : Tot eqtype = x:a{List.memP x lst}
 unfold 
 let fin (#a:eqtype) (lst:list a) = (forall x. List.memP x lst) /\ List.noRepeats lst
 
+(* put helper *)
+
+// let rec put_aux (#t:eqtype) (f:t -> Type) (keys:list t{fin keys}) (ptr:DM.t t (fun x -> B.pointer (f x))) (vmap : DM.t t f) (h : imem (map_inv f ptr keys)) : GTot (imem (map_inv f ptr keys))  = 
+//   let rec aux (ks : list t{List.noRepeats ks}) (h : imem (map_inv f ptr keys){map_inv f ptr ks h})
+//   : GTot (h':imem (map_inv f ptr keys){forall x, ~ List.mem x ks /\ B.live h x => B.get }) = 
+//     match ks with 
+//     | [] -> h 
+//     | k :: ks' ->
+//       let b = DM.sel ptr k in 
+//       let v = DM.sel vmap k in 
+//       let h' = B.g_upd b 0 v h in
+//       (* liveness preservation *)
+//       let _ = g_upd_preserves_map_inv f h b v ptr keys in 
+//       let _ = g_upd_preserves_map_inv f h b v ptr ks' in   
+//       aux ks' h'
+//   in aux keys h
+
+
+//   let rec put_aux (#t:eqtype) (f:t -> Type) (keys:list t{fin keys}) (ptr:DM.t t (fun x -> B.pointer (f x))) (vmap : DM.t t f) (h : imem (map_inv f ptr keys)) : GTot (imem (map_inv f ptr keys))  = 
+//     let rec aux (ks : list t{List.noRepeats ks}) (h : imem (map_inv f ptr keys){map_inv f ptr ks h})
+//     : GTot (h':imem (map_inv f ptr keys){ forall x}) = 
+//       match ks with 
+//       | [] -> h 
+//       | k :: ks' ->
+//         let b = DM.sel ptr k in 
+//         let v = DM.sel vmap k in 
+//         let h' = B.g_upd b 0 v h in
+//         (* liveness preservation *)
+//         let _ = g_upd_preserves_map_inv f h b v ptr keys in 
+//         let _ = g_upd_preserves_map_inv f h b v ptr ks' in   
+//         aux ks' h'
+//     in aux keys h
+
+
 (* Lens constructor *)
 
 (* Try 1 : every element of the type t is in the list *)
@@ -108,22 +151,59 @@ let mk (#t:eqtype) (f:t -> Type) (keys:list t{fin keys}) (ptr:DM.t t (fun x -> B
   let get : get_t (imem (map_inv f ptr keys)) (DM.t t f) = 
     let aux h = 
       let value (k:t) : GTot (f k) =
-      assert (List.memP k keys);
-      let b = DM.sel ptr k in 
-      assume (B.live h b);
-      B.get h b 0
-    in DM.create value in aux
+        let b = DM.sel ptr k in 
+        let _ = map_inv_mem #t f ptr keys h k in 
+        assert (B.live h b);
+        B.get h b 0
+      in DM.create value in aux
+  in 
+  (* First lens law *)
+  let put_property (m : DM.t t f) (h : (imem (map_inv f ptr keys))) (k : t) : Lemma (let b = DM.sel ptr k in B.get (put m h) b 0 == DM.sel m k) =
+    admit ()
   in
-  admit ()
-
+  let get_put_lem (h : (imem (map_inv f ptr keys))) (m : DM.t t f) (k : t) : Lemma (DM.sel (get (put m h)) k == DM.sel m k) = 
+     let h' = put m h in 
+     let _ = put_property m h k in  // main assumption about put
+     let value (k:t) : GTot (f k) =
+       let b = DM.sel ptr k in 
+       let _ = map_inv_mem #t f ptr keys h k in 
+       B.get h' b 0
+     in     
+     let _ = DM.sel_create value k in 
+     assert (DM.sel (get h') k == (let b = DM.sel ptr k in 
+                                   let _ = map_inv_mem #t f ptr keys h k in 
+                                   B.get h' b 0));
+     ()
+  in
+  let get_put_lem_ext (h : (imem (map_inv f ptr keys))) (m : DM.t t f) : Lemma (get (put m h) == m)[SMTPat (get (put m h))] = 
+      forall_intro (get_put_lem h m);
+      DM.equal_elim (get (put m h)) m
+  in
+  // let get_put' () : Lemma (get_put get put) =
+  //   forall_intro_2 #(imem (map_inv f ptr keys)) #(fun _ -> DM.t t f) #(fun h m -> get (put m h) == m) get_put_lem_ext in 
+  let l : imem_lens inv (DM.t t f) fp = { 
+    get = get;
+    put = put;
+    lens_laws = admit () // XXX
+  } in
+  { 
+    footprint = fp;
+    invariant = (fun ptr -> map_inv f ptr keys);
+    x = ptr;
+    snapshot = snap;
+    l = l
+  }
+  
+// Allocation: scoped allocation
+// Experiment: swap with dep map 
+// Get/put with lens composition 
 
 let test1 = 
   fin #(n:nat{n <= 2}) [0;1;2]
 
- 
 (* Idea 2 : the domain of the map is resrticted in the elements of the list *)
 
-let coerce (#a:eqtype) (l : list a) : list (dom #a l) = admit ()
+// let coerce (#a:eqtype) (l : list a) : list (dom #a l) = admit ()
 
-let mk2 (#t:eqtype) (f:t -> Type) (keys:list t) (ptr:DM.t (dom keys) (fun x -> B.pointer (f x))) (h:imem (map_inv f ptr (coerce keys))) 
-: hs_lens (DM.t (dom keys) (fun (x:t) -> B.pointer (f x))) (DM.t (dom keys) f) = admit ()
+// let mk2 (#t:eqtype) (f:t -> Type) (keys:list t) (ptr:DM.t (dom keys) (fun x -> B.pointer (f x))) (h:imem (map_inv f ptr (coerce keys))) 
+// : hs_lens (DM.t (dom keys) (fun (x:t) -> B.pointer (f x))) (DM.t (dom keys) f) = admit ()
